Defined Fifo, NativeFifo, RegFile, and L1Cache based on SinActionT

examples/Fifo.v
@@ -1,6 +1,6 @@
 Require Import Bool String List.
 Require Import Lib.CommonTactics Lib.ilist Lib.Word Lib.Indexer Lib.StringBound.
-Require Import Lts.Syntax Lts.Notations Lts.Semantics Lts.Equiv Lts.Tactics.
+Require Import Lts.Syntax Lts.ParametricSyntax Lts.Notations Lts.Semantics Lts.Equiv Lts.Tactics.
 
 Require Import FunctionalExtensionality Eqdep Eqdep_dec.
 
@@ -68,15 +68,93 @@ Section Fifo.
     with Method ^"deq"() : dType := deq
   }.
 
+  (** SinAction version *)
+  Hypothesis HfifoName: index 0 indexSymbol fifoName = None.
+  Lemma fgn:
+    forall s, index 0 indexSymbol s = None -> index 0 indexSymbol (^s) = None.
+  Proof.
+    pose proof HfifoName.
+    admit.
+  Qed.
+
+  Definition enqS {ty} : forall (d: ty dType), SinActionT ty Void := fun d =>
+    (Read isFull <- { ^"full" | fgn "full" eq_refl };
+     Assert !#isFull;
+     Read elt <- { ^"elt" | fgn "elt" eq_refl };
+     Read enqP <- { ^"enqP" | fgn "enqP" eq_refl };
+     Read deqP <- { ^"deqP" | fgn "deqP" eq_refl };
+     Write { ^"elt" | fgn "elt" eq_refl } <- #elt@[#enqP <- #d];
+     Write { ^"empty" | fgn "empty" eq_refl } <- $$false;
+     LET next_enqP <- (#enqP + $1) :: Bit sz;
+     Write { ^"full" | fgn "full" eq_refl } <- (#deqP == #next_enqP);
+     Write { ^"enqP" | fgn "enqP" eq_refl } <- #next_enqP;
+     Retv)%kami_sin.
+
+  Definition deqS {ty} : SinActionT ty dType :=
+    (Read isEmpty <- { ^"empty" | fgn "empty" eq_refl };
+     Assert !#isEmpty;
+     Read elt <- { ^"elt" | fgn "elt" eq_refl };
+     Read enqP <- { ^"enqP" | fgn "enqP" eq_refl };
+     Read deqP <- { ^"deqP" | fgn "deqP" eq_refl };
+     Write { ^"full" | fgn "full" eq_refl } <- $$false;
+     LET next_deqP <- (#deqP + $1) :: Bit sz;
+     Write { ^"empty" | fgn "empty" eq_refl } <- (#enqP == #next_deqP);
+     Write { ^"deqP" | fgn "deqP" eq_refl } <- #next_deqP;
+     Ret #elt@[#deqP])%kami_sin.
+
+  Definition firstEltS {ty} : SinActionT ty dType :=
+    (Read isEmpty <- { ^"empty" | fgn "empty" eq_refl };
+     Assert !#isEmpty;
+     Read elt : Vector dType sz <- { ^"elt" | fgn "elt" eq_refl };
+     Read deqP <- { ^"deqP" | fgn "deqP" eq_refl };
+     Ret #elt@[#deqP])%kami_sin.
+  
+  Definition fifoS := META {
+    Register { ^"elt" | fgn "elt" eq_refl } : Vector dType sz <- Default
+    with Register { ^"enqP" | fgn "enqP" eq_refl } : Bit sz <- Default
+    with Register { ^"deqP" | fgn "deqP" eq_refl } : Bit sz <- Default
+    with Register { ^"empty" | fgn "empty" eq_refl } : Bool <- true
+    with Register { ^"full" | fgn "full" eq_refl } : Bool <- Default
+
+    with Method { ^"enq" | fgn "enq" eq_refl }(d : dType) : Void := (enqS d)
+    with Method { ^"deq" | fgn "deq" eq_refl }() : dType := deqS
+    with Method { ^"firstElt" | fgn "firstElt" eq_refl }() : dType := firstEltS
+  }.
+
+  Definition simpleFifoS := META {
+    Register { ^"elt" | fgn "elt" eq_refl } : Vector dType sz <- Default
+    with Register { ^"enqP" | fgn "enqP" eq_refl } : Bit sz <- Default
+    with Register { ^"deqP" | fgn "deqP" eq_refl } : Bit sz <- Default
+    with Register { ^"empty" | fgn "empty" eq_refl } : Bool <- true
+    with Register { ^"full" | fgn "full" eq_refl } : Bool <- Default
+
+    with Method { ^"enq" | fgn "enq" eq_refl }(d : dType) : Void := (enqS d)
+    with Method { ^"deq" | fgn "deq" eq_refl }() : dType := deqS
+  }.
+  
 End Fifo.
 
 Hint Unfold fifo simpleFifo : ModuleDefs.
 Hint Unfold enq deq firstElt : MethDefs.
 
+Hint Unfold fifoS simpleFifoS : ModuleDefs.
+Hint Unfold enqS deqS firstEltS : MethDefs.
+
 Section Facts.
   Variable fifoName: string.
   Variable sz: nat.
   Variable dType: Kind.
+
+  Hypothesis HfifoName: index 0 indexSymbol fifoName = None.
+
+  Lemma fifo_fifoS:
+    fifo fifoName sz dType = ParametricSyntax.makeModule (fifoS fifoName sz dType HfifoName).
+  Proof. reflexivity. Qed.
+
+  Lemma simpleFifo_simpleFifoS:
+    simpleFifo fifoName sz dType =
+    ParametricSyntax.makeModule (simpleFifoS fifoName sz dType HfifoName).
+  Proof. reflexivity. Qed.
 
   Lemma fifo_ModEquiv:
     forall m,
