examples/NativeFifo.v
@@ -1,11 +1,12 @@
 Require Import Arith.Peano_dec Bool String List.
 Require Import Lib.CommonTactics Lib.ilist Lib.Word Lib.Indexer Lib.StringBound.
-Require Import Lts.Syntax Lts.Notations Lts.Semantics Lts.Equiv Lts.Tactics.
+Require Import Lts.Syntax Lts.ParametricSyntax Lts.Notations Lts.Semantics Lts.Equiv Lts.Tactics.
 
 Set Implicit Arguments.
 
 Section NativeFifo.
   Variable fifoName: string.
+  
   Variable dType: Kind.
   Variable default: ConstT dType.
 
@@ -65,6 +66,46 @@ Section NativeFifo.
     with Method ^"deq"() : dType := nativeDeq
   }.
 
+  (** SinAction version *)
+  Hypothesis HfifoName: index 0 indexSymbol fifoName = None.
+  Lemma ngn:
+    forall s, index 0 indexSymbol s = None -> index 0 indexSymbol (^s) = None.
+  Proof.
+    pose proof HfifoName.
+    admit.
+  Qed.
+
+  Definition nativeEnqS {ty} : forall (d: ty dType), SinActionT ty Void := fun d =>
+    (ReadN elt : listEltK ty <- { ^"elt" | ngn "elt" eq_refl };
+     Write { ^"elt" | ngn "elt" eq_refl } <- (Var _ (listEltK ty) (listEnq d elt));
+     Retv)%kami_sin.
+
+  Definition nativeDeqS {ty} : SinActionT ty dType :=
+    (ReadN elt : listEltK ty <- { ^"elt" | ngn "elt" eq_refl };
+     Assert !$$(listIsEmpty elt);
+     Write { ^"elt" | ngn "elt" eq_refl } <- (Var _ (listEltK ty) (listDeq elt));
+     Ret (listFirstElt elt))%kami_sin.
+
+  Definition nativeFirstEltS {ty} : SinActionT ty dType :=
+    (ReadN elt : listEltK ty <- { ^"elt" | ngn "elt" eq_refl };
+     Assert !$$(listIsEmpty elt);
+     Ret (listFirstElt elt))%kami_sin.
+  
+  Definition nativeFifoS := META {
+    RegisterN { ^"elt" | ngn "elt" eq_refl } : listEltK type <- (NativeConst nil nil)
+
+    with Method { ^"enq" | ngn "enq" eq_refl } (d : dType) : Void := (nativeEnqS d)
+    with Method { ^"deq" | ngn "deq" eq_refl } () : dType := nativeDeqS
+    with Method { ^"firstElt" | ngn "firstElt" eq_refl } () : dType := nativeFirstEltS
+  }.
+
+  Definition nativeSimpleFifoS := META {
+    RegisterN { ^"elt" | ngn "elt" eq_refl } : listEltK type <- (NativeConst nil nil)
+
+    with Method { ^"enq" | ngn "enq" eq_refl } (d : dType) : Void := (nativeEnqS d)
+    with Method { ^"deq" | ngn "deq" eq_refl } () : dType := nativeDeqS
+  }.
+  
 End NativeFifo.
 
 Hint Unfold nativeFifo nativeSimpleFifo : ModuleDefs.
@@ -72,10 +113,25 @@ Hint Unfold listEltT listEltK listElt
      listIsEmpty listEnq listDeq listFirstElt
      nativeEnq nativeDeq nativeFirstElt: MethDefs.
 
+Hint Unfold nativeFifoS nativeSimpleFifoS : ModuleDefs.
+Hint Unfold nativeEnqS nativeDeqS nativeFirstEltS: MethDefs.
+
 Section Facts.
   Variable fifoName: string.
   Variable dType: Kind.
   Variable default: ConstT dType.
+
+  Hypothesis HfifoName: index 0 indexSymbol fifoName = None.
+
+  Lemma nativeFifo_nativeFifoS:
+    nativeFifo fifoName default =
+    ParametricSyntax.makeModule (nativeFifoS fifoName default HfifoName).
+  Proof. reflexivity. Qed.
+
+  Lemma nativeSimpleFifo_nativeSimpleFifoS:
+    nativeSimpleFifo fifoName default =
+    ParametricSyntax.makeModule (nativeSimpleFifoS fifoName default HfifoName).
+  Proof. reflexivity. Qed.
 
   Lemma nativeFifo_ModEquiv:
     forall m,
